Launchbury/CardinalityAnalysis.thy
@@ -26,8 +26,9 @@ locale CardinalityPrognosisCorrect = CardinalityPrognosis +
   assumes prognosis_Var_thunk: "map_of \<Gamma> x = Some e \<Longrightarrow> ae x = up\<cdot>u \<Longrightarrow> \<not> isLam e \<Longrightarrow> prognosis ae u (delete x \<Gamma>, e, Upd x # S) \<sqsubseteq> record_call x \<cdot> (prognosis ae a (\<Gamma>, Var x, S))"
   assumes prognosis_Var2: "isLam e \<Longrightarrow> x \<notin> domA \<Gamma> \<Longrightarrow> prognosis ae 0 ((x, e) # \<Gamma>, e, S) \<sqsubseteq> prognosis ae 0 (\<Gamma>, e, Upd x # S)"
 
-(*  assumes prognosis_not_called: "prognosis ae a (delete x \<Gamma>, e, S) x = none \<Longrightarrow> ae x = \<bottom> \<Longrightarrow>  prognosis ae a (\<Gamma>, e, S) \<sqsubseteq> prognosis ae a (delete x \<Gamma>, e, S)" *)
-  assumes prognosis_not_called: "ae x = \<bottom> \<Longrightarrow>  prognosis ae a (\<Gamma>, e, S) \<sqsubseteq> prognosis ae a (delete x \<Gamma>, e, S)" 
+  assumes prognosis_not_called: "prognosis ae a (\<Gamma>, e, S) x = none \<Longrightarrow> x \<notin> domA \<Gamma> \<Longrightarrow> prognosis ae a ((x, e') # \<Gamma>, e, S) = prognosis ae a (\<Gamma>, e, S)"
+
+  assumes prognosis_called: "once \<sqsubseteq> prognosis ae a (\<Gamma>, Var x, S) x"
 
 
 
@@ -36,7 +37,8 @@ locale CardinalityPrognosisCorrectLet = CardinalityPrognosisCorrect + Cardinalit
   "atom ` domA \<Delta> \<sharp>* \<Gamma> \<Longrightarrow> atom ` domA \<Delta> \<sharp>* S \<Longrightarrow> edom ae \<subseteq> domA \<Gamma> \<union> upds S \<Longrightarrow> prognosis (Aheap \<Delta> e\<cdot>a \<squnion> ae) a (\<Delta> @ \<Gamma>, e, S) \<sqsubseteq> cHeap \<Delta> e\<cdot>a \<squnion> prognosis ae a (\<Gamma>, Terms.Let \<Delta> e, S)"
 
 locale CardinalityPrognosisEdom = CardinalityPrognosis + CorrectArityAnalysisAheap' +
-  assumes artiy_edom_prognosis: "edom (ABinds \<Gamma>\<cdot>ae \<squnion> Aexp e\<cdot>a) \<subseteq> edom (prognosis ae a (\<Gamma>, e, S))"
+  assumes edom_prognosis:
+    "edom (prognosis ae a (\<Gamma>, e, S)) \<subseteq> fv \<Gamma> \<union> fv e \<union> fv S"
 
 
 end
