Launchbury/FTree-HOLCF.thy
@@ -80,6 +80,9 @@ lemma substitute_mono1': "f \<sqsubseteq> f'\<Longrightarrow> substitute f T t \
 lemma substitute_mono2': "t \<sqsubseteq> t'\<Longrightarrow> substitute f T t \<sqsubseteq> substitute f T t'"
   using  substitute_mono2[folded below_set_def, unfolded paths_mono_iff].
 
+lemma substitute_above_arg: "t \<sqsubseteq> substitute f T t"
+  using  substitute_contains_arg[folded below_set_def, unfolded paths_mono_iff].
+
 lemma and_then_both_single': "and_then x t \<sqsubseteq> both (single x) t"
   using and_then_both_single[folded below_set_def, unfolded paths_mono_iff].
 
